\documentclass[12pt]{article}

\usepackage[margin=1in]{geometry}
\usepackage{amsmath,amsthm,amssymb}
\usepackage{mathrsfs}
\usepackage{mathtools}
\usepackage{enumitem}
\usepackage{physics}

\newcommand{\magsq}[1]{\big|#1\big|^2}
\newcommand{\avg}[1]{\left<#1\right>}
\newcommand{\fullint}{\int_{-\infty}^\infty}
\newcommand{\fullintd}[1]{\fullint\dd#1\:}
\newcommand{\cint}[2]{\int_{#1}^{#2}}
\newcommand{\cintd}[3]{\cint{#1}{#2}\dd#3\:}
\newcommand\treq{\stackrel{\mathclap{\tiny\mbox{Tr}}}{=}}

\begin{document}
	
\title{Exercise Set 3}
\author{Sean Ericson \\ Phys 633}
\maketitle

\section*{Monday}
\subsection*{Exercise 1}
\[ \comm{p^2}{z} = 2i\hbar p_z = -2\hbar^2\partial_z \]

\subsection*{Exercise 2}
\begin{align*}
    \comm{p^2}{r}f &= -\hbar^2\comm{\nabla^2}{r}f \\
    &= -\hbar^2\left(\nabla^2(rf) - r\left(\nabla^2f\right)\right) \\
    &= -\hbar^2\left((\nabla^2r)f + 2(\nabla r)\cdot(\nabla f) + r\nabla^2f - r\nabla^2 f\right) \\
    &= -2\hbar^2\left(\frac{1}{r} - (\nabla r)\cdot\nabla\right)f \\
    &= -2\hbar^2\left(\frac{1}{r} - \hat{r}\cdot\nabla\right)f
\end{align*}
\[ \implies \comm{p^2}{r} = -2\hbar^2\left(\frac{1}{r} - \hat{r}\cdot\nabla\right) \]

\section*{Tuesday}
\subsection*{Exercise 1}
\begin{align*}
    \mathscr{U}_1 &= S_1VP_0 = G_QVP_0 \\
    \mathscr{U}_2 &= S_1VS_1VP_0 + S_2VS_0VP_0 = G_QVG_QVP_0 - G_Q^2VP_0VP_0
\end{align*}


\end{document}