\documentclass[12pt]{article}

\usepackage[margin=1in]{geometry}
\usepackage{amsmath,amsthm,amssymb}
\usepackage{enumitem}
\usepackage{physics}

\newcommand{\magsq}[1]{\big|#1\big|^2}
\newcommand{\avg}[1]{\left<#1\right>}
\newcommand{\fullint}{\int_{-\infty}^\infty}
\newcommand{\fullintd}[1]{\fullint\dd#1\:}
\newcommand{\cint}[2]{\int_{#1}^{#2}}
\newcommand{\cintd}[3]{\cint{#1}{#2}\dd#3\:}

\begin{document}
	
\title{Homework 1}
\author{Sean Ericson \\ Phys 632}
\maketitle

\section*{Problem 1}
Let 
\[ E_s = \hbar\omega_x, \quad t_s = \frac{1}{\omega_x}, \quad x_s = \sqrt{\frac{\hbar}{m\omega_x}}, \quad p_s = \sqrt{m\hbar\omega_x}. \]
\[ \tilde{H} = \frac{H}{E_s}, \quad \tilde{x} = \frac{x}{x_s}, \quad \tilde{y} = \frac{y}{x_s} \quad \tilde{p}_{x(y)} = \frac{p_{x(y)}}{p_s}, \quad \tilde{\omega}_y = \frac{\omega_y}{\omega_x} \]
The Hamiltonian,
\[ H = \frac{1}{2m}\left(p_x^2 + p_y^2\right) + \frac{m}{2}\left(\omega_x^2x^2 + \omega_y^2y^2\right), \]
can then be rewritten as
\[ \tilde{H}E_s = \frac{1}{2m}\left((\tilde{p}_xp_s)^2 + (\tilde{p}_yp_s)^2\right) + \frac{m}{2}\left(\omega_x^2(\tilde{x}x_s)^2 + (\tilde{\omega}_y\omega_x)^2(\tilde{y}x_s)^2\right). \] 
Dropping tildes and substituting in values, this reduces to
\[ H = \frac{1}{2}\left(p_x^2 + p_y^2 + x^2 + \omega_y^2y^2\right) \]


\section*{Problem 2}
In scaled variables,
\begin{align*}
    \partial_t\avg{x} & = -i\avg{\comm{x}{H}} \\
    & = -\frac{i}{2}\avg{\comm{x}{p^2}} \\
    & = \avg{p} \\ \\
    \partial_t\avg{p} & = -i\avg{\comm{p}{H}} \\
    & = -\frac{i}{2}\avg{\comm{p}{x^2}} \\
    & = -\avg{x} \\ \\
    \partial_tV_x & = \partial_t\left(\avg{x^2} - \avg{x}^2\right) \\
    & = -i\avg{\comm{x^2}{H}} - 2\avg{x}\partial_t\avg{x} \\
    & = -\frac{i}{2}\avg{\comm{x^2}{p^2}} - 2\avg{x}\avg{p} \\
    & = 2\avg{\comm{x}{p}_+} - 2\avg{x}\avg{p} \\
    & = 2C_{xp} \\ \\
    \partial_tV_p & = \partial_t\left(\avg{p^2} - \avg{p}^2\right) \\
    & = -i\avg{\comm{p^2}{H}} - 2\avg{p}\partial_t\avg{p} \\
    & = -\frac{i}{2}\avg{\comm{p^2}{x^2}} + 2\avg{x}\avg{p} \\
    & = -2\avg{\comm{x}{p}_+} + 2\avg{x}\avg{p} \\
    & = -2C_{xp} \\ \\
    \partial_tC_{xp} & = \partial_t\left(\avg{\comm{x}{p}_+} - \avg{x}\avg{p}\right) \\
    & = -i\avg{\comm{xp + px}{H}} - \avg{p}^2 + \avg{x}^2 \\
    & = -\frac{i}{2}\avg{\comm{xp}{x^2} + \comm{xp}{p^2} + \comm{px}{x^2} + \comm{px}{p^2}} - \avg{p}^2 + \avg{x}^2 \\
    & = \avg{p^2} - \avg{x^2} - \avg{p}^2 + \avg{x}^2 \\
    & = V_p - V_x 
\end{align*}
Restoring units,
\begin{align*}
    \partial_t\avg{x} & = \frac{1}{m}\avg{p} \\
    \partial_t\avg{p} & = -m\omega^2\avg{x} \\
    \partial_tV_x & = \frac{2}{m}C_{xp} \\
    \partial_tV_P & = -m\omega^2C_{xp} \\
    \partial_tC_{xp} & = \frac{1}{m}V_p - m\omega^2V_x
\end{align*}


\section*{Problem 3}
From the result of Homework 3 Problem 3 from last term,
\[ V_x(t) = \sigma^2(t) = \sigma^2 + \frac{\hbar^2t^2}{4m^2\sigma^2} \]
\[ \implies \dot{V}_x(t) = \frac{\hbar^2t}{2m^2\sigma^2} \]
Using the equations from problem 2 above (with $\omega = 0$) we see that
\[ \partial_tV_p = 0 \implies V_p = c \]
for some constant $c$. This implies that the time dependence of $C_{xp}$ has the simple form 
\[ C_{xp}(t) = \frac{c}{m}t + k \]
for another constant $k$, which in turn implies
\[ V_x(t) = V_x(0) + \frac{c}{m^2}t \]
The substituting in the initial conditions gives
\[ V_x(t) = \sigma^2 + \frac{\hbar^2t^2}{4m^2\sigma^2} \]


\section*{Problem 4}
Let 
\[ U_g = V_x V_p - C_{xp}^2 \]
Then
\begin{align*}
    \partial_tU_g & = \dot{V}_xV_p + V_x\dot{V}_p - 2C_{xp}\dot{C}_{xp} \\
    & = 2C_{xp}V_p -2C_{xp}V_x - 2C_{xp}(V_p-V_x) \\
    & = 2C_{xp}(V_p - V_x - V_p + V_x) \\
    & = 0
\end{align*}

\end{document}